# â„–1

$\frac{d}{d\eta} \int_{-\infty}^\infty p(y, \eta) dy = \int_{-\infty}^\infty \frac{d}{d\eta} b(y) exp(\eta y - \alpha(\eta))dy = \int_{-\infty}^\infty b(y) (y-\frac{d}{d\eta} \alpha(\eta)) exp(\eta y - \alpha(\eta))dy = \int_{-\infty}^\infty y p(y, \eta) - \alpha(\eta) \int_{-\infty}^\infty p(y, \eta)dy$

$[\int_{-\infty}^\infty y p(y, \eta)dy = E[Y, \eta]; \int_{-\infty}^\infty p(y, \eta)dy = 1; \frac{d}{d\eta} \int_{-\infty}^\infty p(y, \eta) dy = 0]$

$E[Y, \eta] - \frac{d}{d\eta} \alpha(\eta) = 0$

$E[Y, \eta] = \frac{d}{d\eta} \alpha(\eta)$

# â„–2

$\int_{-\infty}^\infty b(y) exp(\eta y - \alpha(\eta))dy = 1 | * exp(\alpha(\eta))$

$\int_{-\infty}^\infty b(y) exp(\eta y)dy = exp(\alpha(\eta)) | \frac{d}{d\eta}$

$\int_{-\infty}^\infty y b(y) exp(\eta y)dy = \frac{d}{d\eta} \alpha(\eta) exp(\alpha(\eta)) | \frac{d}{d\eta}$

$\int_{-\infty}^\infty y^2 b(y) exp(\eta y)dy = \frac{d^2}{d\eta^2} \alpha(\eta) exp(\alpha(\eta)) + (\frac{d}{d\eta} \alpha(\eta))^2 exp(\alpha(\eta))| * exp(-\alpha(\eta))$

$\int_{-\infty}^\infty y^2 p(y, \eta) dy = \frac{d^2}{d\eta^2} \alpha(\eta) + (\frac{d}{d\eta} \alpha(\eta))^2$

$Var(y; \eta)=E[y^2, \eta]-(E[y, \eta])^2=\int_{-\infty}^\infty y^2 p(y, \eta) dy - (\frac{d}{d\eta} \alpha(\eta))^2 = \frac{d^2}{d\eta^2} \alpha(\eta)$

# â„–3

$ln(\prod_{k=1}^{m} b(y^{(k)}) exp( \theta^T x^{k} y^{k} - \alpha(\theta^T x^{k}) ))=$
$-\sum_{k=1}^m ln( b(y^{(k)}) ) -\sum_{k=1}^m(\theta^T x^{k} y^{k} - \alpha(\theta^T x^{k}))=l(\theta)$

$\frac{d^2}{d\theta_j d\theta_i}l(\theta)=$
$\sum_{k=1}^m \frac{d^2}{d\eta^2} \frac{d\eta}{d\theta_j} \frac{d\eta}{d\theta_i} \alpha(\theta^T x^{k})=$
$\sum_{k=1}^m x_i^{(k)} x_j^{(k)} Var[y^{(k)} | x^{(k)}; \theta]$

$H(\theta) = \sum_{i=1}^n \sum_{j=1}^n \frac{d^2}{d\theta_j d\theta_i}l(\theta) \theta_i \theta_j =$
$\sum_{i=1}^n \sum_{j=1}^n\theta_i \theta_j \sum_{k=1}^m x_i^{(k)} x_j^{(k)} Var[y^{(k)} | x^{(k)}; \theta]=$
$\sum_{k=1}^m Var[y^{(k)} | x^{(k)}; \theta] \sum_{i=1}^n \theta_i x_i^{(k)} \sum_{j=1}^n \theta_j x_j^{(k)} \ge 0$

Because: 

$Var[y^{(k)} | x^{(k)}; \theta] \ge 0$

$\sum_{j=1}^n \theta_j x_j^{(k)} = \sum_{i=1}^n \theta_i x_i^{(k)} =>$
$\sum_{i=1}^n \theta_i x_i^{(k)} \sum_{j=1}^n \theta_j x_j^{(k)} = (\sum_{i=1}^n \theta_i x_i^{(k)})^2 \ge 0$
