# 3

$p(t^{(i)}=1|y^{(i)}=1, x^{(i)}) = $
$\frac{p(y^{(i)}=1|t^{(i)}=1, x^{(i)})p(t^{(i)}=1 |x^{(i)})}{p(y^{(i)}=1| x^{(i)})}=$
$\frac{p(y^{(i)}=1|t^{(i)}=1, x^{(i)})p(t^{(i)}=1 |x^{(i)})}{p(y^{(i)}=1|t^{(i)}=0, x^{(i)})*p(t^{(i)}=0 |x^{(i)}) + p(y^{(i)}=1|t^{(i)}=1, x^{(i)})*p(t^{(i)}=1 |x^{(i)})}=$
$\frac{1}{1+\frac{p(y^{(i)}=1|t^{(i)}=0, x^{(i)})*p(t^{(i)}=0 |x^{(i)})}{p(y^{(i)}=1|t^{(i)}=1, x^{(i)})*p(t^{(i)}=1 |x^{(i)})}} = 1$

Because

$p(y^{(i)}=1|t^{(i)}=0, x^{(i)}) = 0$

# 4

$1=\frac{\alpha p(t^{(i)}=1|x^{(1)})}{p(y^{(i)}=1|x^{(i)})}$

$ p(t^{(i)}=1|x^{(i)})=\frac{1}{\alpha}p(y^{(i)}=1|x^{(i)})$

# 5

$E[h(x^{(i)})|y^{(i)}=1]=E[p(y^{(i)}=1|x^{(i)})|y^{(i)}=1]=\alpha p(y^{(i)}=1| x^{(i)}, y^{(i)}=1)=\alpha$
