<div style="text-align: center;">

# № 1

$\theta_{MAP}=argmax_{\theta}\ p(\theta|x,y)=$

$argmax_{\theta}\frac{p(x, y|\theta)p(\theta|x)}{p(x,y)}=$

$[p(\theta)=p(\theta|x);\ p(x,y)\ не\ зависит от\ \theta,\ следовательно,\ не\ влияет\ на\ argmax]=$

$argmax_{\theta}\ p(x,y|\theta)p(\theta)=$

$argmax_{\theta}\ p(x, y, \theta)=$

$argmax_{\theta}\ p(y|x,\theta)p(x, \theta)=$

$argmax_{\theta}\ p(y|x,\theta)p(\theta)$

# № 2

$\theta_{MAP}=argmax_{\theta}p(y|x,\theta)p(\theta)=$

$argmin_{\theta}(-log\ p(y|x,\theta)p(\theta))=$

$argmin_{\theta}(-log\ p(y|x,\theta) - log\ p(\theta))=$

$argmin_{\theta}(-log\ p(y|x,\theta) - (log\ p(\theta_1) +..+ log\ p(\theta_n)))=$

$argmin_{\theta}(-log\ p(y|x,\theta) - (log\ \sum_{i=1}^n \frac{1}{\eta\sqrt{2\pi}}e^{-0.5\ (\frac{\theta_i}{\eta})^2}))=$

$argmin_{\theta}(-log\ p(y|x,\theta)+\sum_{i=1}^n0.5\ (\frac{\theta_i^2}{\eta^2}))$

$[\lambda =\frac{1}{2\eta^2}]$

$\theta_{MAP}=argmin_{\theta}(-log\ p(y|x,\theta)+\lambda\theta^2_1+..+\lambda\theta^2_n)$

## 

$\theta_{MLE}=argnmin_{\theta}(-log\ p(y|x,\theta)+\lambda||\theta||^2_2)=$
$argnmin_{\theta}(-log\ p(y|x,\theta)+\lambda\theta^2_1+..+\lambda\theta^2_n)$

# № 3

$p(\theta|x,y)=p(y|x,\theta)p(\theta)$

$log\ p(\theta|x,y)=log\ p(y|x,\theta)\ log\ p(\theta)=$

$log\ p(y|x,\theta)-\sum_{i=1}^n\frac{\theta^2}{2\eta^2}-n\ log\ \eta\sqrt{2\pi}$

$\frac{d\ log\ p(\theta|x,y))}{d\  \theta}=-\frac{\theta}{2\eta^2}$

##

$(log \frac{1}{\eta\sqrt{2\pi}}e^{-\frac{\theta^2}{2\eta^2}})^`_\theta=$
$(-\frac{\theta^2}{2\eta^2}+log \frac{1}{\eta\sqrt{2\pi}})^`_\theta=$
$\frac{-1}{\eta^2}\theta^T$

$y-\theta^Tx\in N(0, \sigma^2)$ =>
$y\in N(\theta^Tx, \sigma^2)$

##

$p(y|x,\theta)=\prod_{i=1}^m p(y^{(i)}|x^{(i)},\theta)=$
$\prod_{i=1}^m \frac{1}{\sigma^2\sqrt{2\pi}}e^{-\frac{(y^{(i)}-\theta^Tx^{(i)})^2}{2\sigma^2}}$

$log\ p(y|x,\theta)=-\frac{1}{2\sigma^2}\sum_{i=1}^m (y^{(i)}-\theta^Tx^{(i)})^2+const=$

$-\frac{1}{2\sigma^2} (y-\theta^Tx)^T(y-\theta^Tx) + const=$

$-\frac{1}{2\sigma^2} ||(y-\theta^Tx)||^2_2 + const=$

$\frac{d\ log\ p(y|x,\theta)}{d\  \theta}=-\frac{1}{2\sigma^2}(2y^Tx-2\theta^Tx^Tx)=0$

$\theta^Tx^Tx=y^Tx$

$\theta^T=y^Tx(x^Tx)^{-1}$

$\theta_{MLE}=(x^Tx)^{-1}x^Ty$

##

$(y^{(i)}-\theta^Tx^{(i)})^`_\theta=(yy-2y\theta^Tx+(\theta^Tx)^2)^`_\theta=-2y^Tx+2\theta^Tx^Tx$

##  

$\frac{d\ log\ p(\theta|x,y)}{d\  \theta}=\frac{1}{\sigma^2}(y^Tx-\theta^Tx^Tx)-\frac{1}{n^2}\theta^T=0$

$y^Tx=\theta^Tx^Tx-\frac{\sigma^2}{n^2}\theta^T$

$\theta^T(x^Tx+\frac{\sigma^2}{n^2}I)=y^Tx$

$\theta^T=y^Tx(x^Tx+\frac{\sigma^2}{n^2}I)^{-1}$

$\theta_{MAP}=(x^Tx+\frac{\sigma^2}{n^2}I)^{-1}yx^T$

# № 4

$\theta_{MAP}=argmax_{\theta}p(y|x,\theta)p(\theta)=$

$argmin_{\theta}(-log\ p(y|x,\theta) - log\ p(\theta))=$

$argmin_{\theta}(-log\ p(y|x,\theta) - (log\ p(\theta_1) +..+ log\ p(\theta_n)))=$

$argmin_{\theta}(-log\ p(y|x,\theta) - \sum_{i=1}^n \frac{|\theta_i|}{b} - log\ 2b)=$

$argmin_{\theta}(-log\ p(y|x,\theta) - \frac{||\theta||}{b})$

## 

$p(y|x,\theta)=\prod_{i=1}^m p(y^{(i)}|x^{(i)},\theta)=$
$\prod_{i=1}^m \frac{1}{\sigma^2\sqrt{2\pi}}e^{-\frac{(y^{(i)}-\theta^Tx^{(i)})^2}{2\sigma^2}}$

$log\ p(y|x,\theta)=-\frac{1}{2\sigma^2}\sum_{i=1}^m (y^{(i)}-\theta^Tx^{(i)})^2+const=$

$-\frac{1}{2\sigma^2} ||(y-\theta^Tx)||^2_2 + const$

## 

$\theta_{MAP}=argmin_{\theta}(\frac{1}{2\sigma^2} ||(y-\theta^Tx)||^2_2+\frac{1}{b}||\theta||)=$

$argmin_{\theta}(||(y-\theta^Tx)||^2_2+\frac{2\sigma^2}{b}||\theta||)=$

$[\gamma=\frac{2\sigma^2}{b}]$

</div>